\section{Technical Appendix}

%%%  PUBLIC ANNOUNCEMENTS

\begin{lemma}\label{lem:palproperties} The following equalities hold:
\begin{enumerate}
\item $\truthset{\modults}{\gann{\chi}\varphi} = \truthset{\modults}{\neg\chi} \cup \truthset{\annmodelchi}{\varphi}$.
\item $\truthset{\annmodelchi}{\varphi} = \truthset{\modults}{\chi \wedge \gann{\chi}\varphi}$.
\end{enumerate}
\end{lemma}

\begin{proof}
\ 
\begin{enumerate}
\item Let $w \in \truthset{\modults}{\gann{\chi}\varphi}$, we have that $\modults,w \models \gann{\chi}\varphi$. Thus, $\modults,w \models \chi$ implies $\annmodelchi,w \models \varphi$, which it can be rewritten as $\modults,w \models \neg\chi$ or $\annmodelchi,w \models \varphi$. Hence, $w \in \truthset{\modults}{\neg\chi} \cup \truthset{\annmodelchi}{\varphi}$. The other inclusion behaves the same way.
\item Let $w \in \truthset{\annmodelchi}{\varphi}$, we have that $w \in \annsemantics{\W}{\chi} = \truthset{\modults}{\chi}$ and $w \in \truthset{\annmodelchi}{\varphi}$. Thus, $w \in \truthset{\modults}{\chi} \cap \truthset{\annmodelchi}{\varphi}$. The previous set is in the form of $(A \cap B)$. By set reasoning, it is equal to $(A \cap (A^c \cup B))$.
In other words, it is equivalent to $w \in \truthset{\modults}{\chi} \cap (\truthset{\modults}{\neg\chi} \cup \truthset{\annmodelchi}{\varphi})$. Using the result of the first item, $w \in \truthset{\modults}{\chi} \cap \truthset{\modults}{\gann{\chi}\varphi}$. Hence, $w \in \truthset{\modults}{\chi \wedge \gann{\chi}\varphi}$.
The other inclusion behaves the same way.
\end{enumerate}
\end{proof}

\begin{lemma}
The reduction axioms from~\Cref{tab:palaxiom} are valid in $\cultsba$.
\end{lemma}

\begin{proof} The proof proceeds by cases:
\begin{itemize}
\item For \axm{RAtom}, suppose $\modults,w \models \chi$. Then $\annmodelchi,w \models p$ iff $p \in \annsemantics{\V}{\chi}(w)$. Since $\annsemantics{\V}{\chi}(w) = \V(w)$, we have that $\modults,w \models p$.
By definition, $\modults,w \models \gann{\chi}p$ iff $\modults,w \models \chi$ then $\annmodelchi,w \models p$, which is equivalent to $\modults,w \models \chi$ then $\modults,w \models p$.
Thus, equivalent to $\modults,w \models (\chi \implies p)$.

\item For \axm{R$\neg$}, by definition $\modults,w \models (\chi \implies \neg\gann{\chi}\varphi)$ iff $\modults,w \models \chi$ implies $\modults,w \models \neg\gann{\chi}\varphi$.
Again, by definition $\modults,w \models \neg\gann{\chi}\varphi$ iff $\modults,w \models \chi$ and $\annmodelchi,w \not\models \varphi$.
Thus, $\modults,w \models (\chi \implies \neg\gann{\chi}\varphi)$ iff $\modults,w \models \chi$ implies $\modults,w \models \chi$ and $\annmodelchi,w \not\models \varphi$.
The previous implication is in the form of $(A \implies (A \wedge B))$.
By propositional reasoning, this is equivalent to $(A \implies B)$.
In other words, it is equivalent to $\modults,w \models \chi$ implies $\annmodelchi,w \not\models \varphi$.
Since, $\annmodelchi,w \not\models \varphi$ iff $\annmodelchi,w \models \neg\varphi$, by the definition of $\gann{\chi}$, we have that $\modults,w \models \gann{\chi}\neg\varphi$.

\item For \axm{R$\vee$}, by definition of $\gann{\chi}$ we have that $\modults,w \models \gann{\chi}(\varphi \vee \psi)$ iff $\modults,w \models \chi$ implies $\annmodelchi,w \models \varphi \vee \psi$. Which is equivalent to $\modults,w \models \chi$ implies $\annmodelchi,w \models \varphi$ or $\annmodelchi,w \models \psi$.
The previous implication is in the form of $(A \implies (B \vee C))$. By propositional reasoning, this is equivalent to $((A \implies B) \vee (A \implies C))$.
In other words, it is equivalent to $\modults,w \models \chi$ implies $\annmodelchi,w \models \varphi$, or $\modults,w \models \chi$ implies $\annmodelchi,w \models \psi$.
By the definition of $\gann{\chi}$, $\modults,w \models \gann{\chi}\varphi$ or $\modults,w \models \gann{\chi}\psi$ and thus $\modults,w \models \gann{\chi}\varphi \vee \gann{\chi}\psi$.

\item For \axm{RKh}, by the definition of $\gann{\chi}$, $\modults,w \models \gann{\chi}\khi(\varphi,\psi)$ iff $\modults,w \models \chi$ implies $\annmodelchi,w \models \khi(\varphi,\psi)$. Using the definition of $\khi$, $\annmodelchi,w \models \khi(\varphi,\psi)$ iff there is $\plans \in (\annsemantics{\Unc}{\chi})(i)$ with $\plans \subseteq \ACT$ s.t. $\truthset{\annmodelchi}{\varphi} \subseteq \stexec^{\annmodelchi}(\plans)$ and $(\annsemantics{\R}{\chi})_\plans(\truthset{\annmodelchi}{\varphi}) \subseteq \truthset{\annmodelchi}{\psi}$.
By the definition of $\annmodelchi$, $(\annsemantics{\Unc}{\chi})(i)=\Unc(i)$. Using \Cref{lem:palproperties}, $\truthset{\annmodelchi}{\varphi} = \truthset{\modults}{\chi \wedge \gann{\chi}\varphi}$ and $\truthset{\annmodelchi}{\psi} = \truthset{\modults}{\chi \wedge \gann{\chi}\psi}$.
Thus, $\annmodelchi,w \models \khi(\varphi,\psi)$ iff there is $\plans \in \Unc(i)$ with $\plans \subseteq \ACT$ s.t. $\truthset{\modults}{\chi \wedge \gann{\chi}\varphi} \subseteq \stexec^{\annmodelchi}(\plans)$ and $(\annsemantics{\R}{\chi})_\plans(\truthset{\modults}{\chi \wedge \gann{\chi}\varphi}) \subseteq \truthset{\modults}{\chi \wedge \gann{\chi}\psi}$.
Let $a \in \plans$ and $w \in \annsemantics{\W}{\chi}$. If $w \in \truthset{\modults}{\chi \wedge \gann{\chi}\varphi}$, then:
\begin{itemize}
    \item $(\annsemantics{\R}{\chi})_a(w) \neq \emptyset$ (since $w \in \stexec^{\annmodelchi}(a)$) and
    \item $(\annsemantics{\R}{\chi})_a(w) \subseteq \truthset{\modults}{\chi \wedge \gann{\chi}\psi}$.
\end{itemize}
Using \Cref{def:annupdate}, the first item is equivalent to $w \in \truthset{\modults}{\chi}$, $\R_a(w) \subseteq \truthset{\modults}{\chi}$ and $\R_a(w) \neq \emptyset$ and with this information, $(\annsemantics{\R}{\chi})_a(w) = \R_a(w)$ that is useful for the second item.
Hence, if $w \in \truthset{\modults}{\chi \wedge \gann{\chi}\varphi}$, then:
\begin{itemize}
    \item $w \in \truthset{\modults}{\chi}$, $\R_a(w) \subseteq \truthset{\modults}{\chi}$ and $\R_a(w) \neq \emptyset$ and
    \item $\R_a(w) \subseteq \truthset{\modults}{\chi \wedge \gann{\chi}\psi}$.
\end{itemize}
Note that $w \in \truthset{\modults}{\chi}$ and $\R_a(w) \subseteq \truthset{\modults}{\chi}$ are redundant as $w \in \truthset{\modults}{\chi \wedge \gann{\chi}\varphi}$ and $\R_a(w) \subseteq \truthset{\modults}{\chi \wedge \gann{\chi}\psi}$.
With this, if $w \in \truthset{\modults}{\chi \wedge \gann{\chi}\varphi}$, then:
\begin{itemize}
    \item $\R_a(w) \neq \emptyset$ (thus, $w \in \stexec^\modults(a)$) and
    \item $\R_a(w) \subseteq \truthset{\modults}{\chi \wedge \gann{\chi}\psi}$.
\end{itemize}
Since we prove for arbitrary $a \in \plans$ and $w \in \annsemantics{\W}{\chi}$, the result yields for all $a \in \plans$ and $w \in \annsemantics{\W}{\chi}$.
Moreover, it can be generalized for all $w \in \W$ as if $w \in \truthset{\modults}{\chi \wedge \gann{\chi}\varphi}$, then $w \in \annsemantics{\W}{\chi}$; and if $w \in \annsemantics{\W}{\chi}$, then $w \in \W$.
Now $\annmodelchi,w \models \khi(\varphi,\psi)$ iff there is $\plans \in \Unc(i)$ with $\plans \subseteq \ACT$ s.t. $\truthset{\modults}{\chi \wedge \gann{\chi}\varphi} \subseteq \stexec(\plans)$ and $\R_\plans(\truthset{\modults}{\chi \wedge \gann{\chi}\varphi}) \subseteq \truthset{\modults}{\chi \wedge \gann{\chi}\psi}$.
This happens iff $\modults,w \models \khi(\chi \wedge \gann{\chi}\varphi,\chi \wedge \gann{\chi}\psi)$. Since for this equivalence we prove assuming $\modults,w \models \chi$, then $\modults,w \models \chi$ implies $\annmodelchi,w \models \khi(\varphi,\psi)$ iff $\modults,w \models \chi$ implies $\modults,w \models \khi(\chi \wedge \gann{\chi}\varphi,\chi \wedge \gann{\chi}\psi)$. Thus, iff $\modults,w \models \chi \implies \khi(\chi \wedge \gann{\chi}\varphi,\chi \wedge \gann{\chi}\psi)$.
\end{itemize}
\end{proof}



%% ARROW UPDATES 

\begin{lemma}
The reduction axioms from \Cref{tab:aulaxiom} are valid.
\end{lemma}

\begin{proof} The proof proceeds by cases:
\begin{itemize}
\item For \axm{RBase}, let $U' = (\bigwedge_{i=1}^n \theta_i,\bigwedge_{i=1}^n \theta'_i) = (\alpha_1,\theta'_1)$, note that $\arrowsemantics{\W}{U} = \arrowsemantics{\W}{U'} = \W$, $\arrowsemantics{\Unc}{U} = \arrowsemantics{\Unc}{U'} = \Unc$ and $\arrowsemantics{\V}{U}(p) = \arrowsemantics{\V}{U'}(p) = \V(p)$ for every $p$. Let $a \in \ACT$, $(w,v) \in (\arrowsemantics{\R}{U})_a$ iff $w \in \truthset{\modults}{\bigwedge_{i=1}^n \theta_i}$, $\R_a(w) \subseteq \truthset{\modults}{\bigwedge_{i=1}^n \theta'_i}$.
Since $\truthset{\modults}{\bigwedge_{i=1}^n \theta_i} = \truthset{\modults}{\alpha_1} = \truthset{\modults}{\bigwedge_{i=1}^1 \alpha_i}$ and $\truthset{\modults}{\bigwedge_{i=1}^n \theta'_i} = \truthset{\modults}{\theta'_1} = \truthset{\modults}{\bigwedge_{i=1}^1 \theta'_i}$, $(w,v) \in (\arrowsemantics{\R}{U})_a$ iff $(w,v) \in (\arrowsemantics{\R}{U'})_a$.
With this, $(\arrowsemantics{\R}{U})_a = (\arrowsemantics{\R}{U'})_a$ for all $a \in \ACT$, $\arrowmodelU = \arrowmodel{U'}$ and satisfy the same formulas.
Thus, $\modults,w \models \arrowdiam{U}\varphi$ iff $\modults,w \models \arrowdiam{U'}\varphi$.

\item For \axm{RAtom}, let $U = (\theta,\theta')$, $\modults,w \models \arrowdiam{U}p$ iff $\arrowmodelU,w \models p$. Since $\arrowsemantics{\V}{U}(w) = \V(w)$, $p \in \arrowsemantics{\V}{U}(w)$ iff $w \in \V(p)$. Thus, $\modults,w \models \arrowdiam{U}p$ iff $\modults,w \models p$.

\item For \axm{R$\neg$}, let $U = (\theta,\theta')$, $\modults,w \models \arrowdiam{U}\neg\varphi$ iff $\arrowmodelU,w \models \neg\varphi$ iff $\arrowmodelU,w \not\models \varphi$ iff $\modults,w \not\models \arrowdiam{U}\varphi$ iff $\modults,w \models \neg\arrowdiam{U}\varphi$.

\item For \axm{R$\vee$}, let $U = (\theta,\theta')$,
$\modults,w \models \arrowdiam{U}(\varphi \vee \psi)$ iff $\arrowmodelU,w \models \varphi \vee \psi$ iff $\arrowmodelU,w \models \varphi$ or $\arrowmodelU,w \models \psi$ iff $\modults,w \models \arrowdiam{U}\varphi$ or $\modults,w \models \arrowdiam{U}\psi$ iff $\modults,w \models \arrowdiam{U}\varphi \vee \arrowdiam{U}\psi$.

\item For \axm{RKh}, let $U = (\theta,\theta')$, by the definition of $\arrowdiam{U}$, $\modults,w \models \arrowdiam{U}\khi(\varphi,\psi)$ iff $\arrowmodelU,w \models \khi(\varphi,\psi)$.
Using the definition of $\khi$, $\arrowmodelU,w \models \khi(\varphi,\psi)$ iff there is $\plans \in (\arrowsemantics{\Unc}{U})_i$ with $\plans \subseteq \ACT$ s.t. $\truthset{\arrowmodelU}{\varphi} \subseteq \stexec^{\arrowmodelU}(\plans)$ and $\R'_\plans(\truthset{\arrowmodelU}{\varphi}) \subseteq \truthset{\arrowmodelU}{\psi}$.
By the definition of $\arrowmodelU$, $(\arrowsemantics{\Unc}{\chi})_i=\Unc(i)$. Using the definition of $\arrowdiam{U}$, $\truthset{\arrowmodelU}{\varphi} = \truthset{\modults}{\arrowdiam{U}\varphi}$ and $\truthset{\arrowmodelU}{\psi} = \truthset{\modults}{\arrowdiam{U}\psi}$.
Thus, $\arrowmodelU,w \models \khi(\varphi,\psi)$ iff there is $\plans \in \Unc(i)$ with $\plans \subseteq \ACT$ s.t. $\truthset{\modults}{\arrowdiam{U}\varphi} \subseteq \stexec^{\arrowmodelU}(\plans)$ and $\R'_\plans(\truthset{\modults}{\arrowdiam{U}\varphi}) \subseteq \truthset{\modults}{\arrowdiam{U}\psi}$.
Let $a \in \plans$ and $w \in \arrowsemantics{\W}{U}$. If $w \in \truthset{\modults}{\arrowdiam{U}\varphi}$, then:
\begin{itemize}
\item $(\arrowsemantics{\R}{U})_a(w) \neq \emptyset$ (since $w \in \stexec^{\arrowmodelU}(a)$) and
\item $(\arrowsemantics{\R}{U})_a(w) \subseteq \truthset{\modults}{\arrowdiam{U}\psi}$.
\end{itemize}
Using \Cref{def:arrowupdate}, the first item is equivalent to $w \in \truthset{\modults}{\theta}$, $\R_a(w) \subseteq \truthset{\modults}{\theta'}$ and $\R_a(w) \neq \emptyset$ and with this information, $(\arrowsemantics{\R}{U})_a(w) = \R_a(w)$ that is useful for the second item.
Hence, if $w \in \truthset{\modults}{\arrowdiam{U}\varphi}$, then:
\begin{itemize}
\item $w \in \truthset{\modults}{\theta}$,
\item $\R_a(w) \neq \emptyset$ (thus, $w \in \stexec^\modults(a)$),
\item $\R_a(w) \subseteq \truthset{\modults}{\theta'}$ and $\R_a(w) \subseteq \truthset{\modults}{\arrowdiam{U}\psi}$.
\end{itemize}
Since the first item is independent from $\plans$, we can put it outside of the expression.
With some minor adjustments we have that $\modults,w \models \A(\arrowdiam{U}\varphi \implies \theta)$ and if $w \in \truthset{\modults}{\arrowdiam{U}\varphi}$, then:
\begin{itemize}
\item $\R_a(w) \neq \emptyset$ (thus, $w \in \stexec^\modults(a)$),
\item $\R_a(w) \subseteq \truthset{\modults}{\theta' \wedge \arrowdiam{U}\psi}$.
\end{itemize}

Since we prove for arbitrary $a \in \plans$ and $w \in \arrowsemantics{\W}{U} = \W$, the result yields for all $a \in \plans$ and $w \in \arrowsemantics{\W}{U} = \W$.
Now $\arrowmodelU,w \models \khi(\varphi,\psi)$ iff $\modults,w \models \A(\arrowdiam{U}\varphi \implies \theta)$ and there is $\plans \in \Unc(i)$ with $\plans \subseteq \ACT$ s.t. $\truthset{\modults}{\arrowdiam{U}\varphi} \subseteq \stexec(\plans)$ and $\R_\plans(\arrowdiam{U}\varphi) \subseteq \truthset{\modults}{\theta' \wedge \arrowdiam{U}\psi}$.
This happens iff $\modults,w \models (\A(\arrowdiam{U}\varphi \implies \theta) \wedge \khi(\arrowdiam{U}\varphi,\theta' \wedge \arrowdiam{U}\psi))$ with $U = (\theta,\theta')$.
\end{itemize}
\end{proof}

